restructuring proof...

modules/clide-collaboration/src/main/isabelle/clide/collaboration/Operation.thy
@@ -1,98 +1,199 @@
-theory Operation
-imports Main List Option Set SimpleOperation 
-begin
+(* Formalisation of Operational Transformation *)
+(* author: Martin Ring, DFKI Bremen *) (*<*) 
 
-datatype 'char action = Retain nat | Insert "'char list" | Delete nat
+theory Operation
+imports Main List Option Set
+begin (*>*)
+
+section {* Actions, Operations and Documents *}
+
+text {* A @{term document} is a list of elements. *}
+
+type_synonym 'char document = "'char list"
+
+text {* An @{term action} can either alter the document at the current position or move the virtual 
+        cursor on the document forward or do both. *}
+
+datatype 'char action = Retain nat | Insert 'char "'char list" | Delete nat
+
+text {* An @{term operation} is a list of actions. *}
 
 type_synonym 'char operation = "'char action list"
 
-text {* We define an inductive set of all operations and their equivalent simple operations *}
+text {* There are three types of actions of which an operation is composed:
+        @{term Retain}, @{term "Insert c"} and @{term Delete}. An operation is
+        a list of actions.
 
-inductive_set operations :: "('char SimpleOperation.operation \<times> 'char operation) set" where
-  empty[intro!]:  "([],[]) \<in> operations"
-| retain[intro!]: "(a,b) \<in> operations \<Longrightarrow> (append (List.replicate n SimpleOperation.Retain) a, Retain n#b) \<in> operations"
-| insert[intro!]: "(a,b) \<in> operations \<Longrightarrow> (append (List.map SimpleOperation.Insert s) a, Insert s#b) \<in> operations"
-| delete[intro!]: "(a,b) \<in> operations \<Longrightarrow> (append (List.replicate n SimpleOperation.Delete) a, Delete n#b) \<in> operations"
+        \begin{itemize}
+          \item @{term "Retain n"} moves the cursor @{term "n + 1"} positions forward, not altering 
+                                   the text.
+          \item @{term "Insert c cs"} inserts elements in @{term "c#cs"} at the position of the cursor 
+                                      and moves the cursor behind these elements.
+          \item @{term "Delete n"} deletes the next @{term "n + 1"} elements of the document, not 
+                                   moving the cursor.
+        \end{itemize} *}
 
-lemma singleRetain: "a \<in> Domain operations \<Longrightarrow> SimpleOperation.Retain#a \<in> Domain operations"
-  sorry
+subsection {* In- and Output Lengths of Operations *}
 
-lemma singleInsert: "a \<in> Domain operations \<Longrightarrow> SimpleOperation.Insert c#a \<in> Domain operations"
-  sorry
+text {* An operation has an input length and an output length:
 
-lemma singleDelete: "a \<in> Domain operations \<Longrightarrow> SimpleOperation.Delete#a \<in> Domain operations"
-  sorry
+        \begin{itemize}
+          \item The input length is the length of a document on which the operation can
+                be applied.
+          \item The output length is the length of the result of the application on a
+                document on which the operation is defined.
+        \end{itemize} *}
 
+fun inputLength :: "'char operation \<Rightarrow> nat" where
+  "inputLength [] = 0"
+| "inputLength (Retain n#xs) = (1 + n) + inputLength xs"
+| "inputLength (Insert c cs#xs) = inputLength xs"
+| "inputLength (Delete n#xs) = (1 + n) + inputLength xs"
 
-lemma operationsComplete1: "a \<in> Domain operations"
-  apply (induct_tac a, force)
-  apply (case_tac a, auto simp add: singleRetain singleInsert singleDelete)
+text {* if an operation @{term a} has input lenght 0, a must be empty or it consists only of insert 
+        actions *}
+
+lemma emptyInputInsert [rule_format]: "inputLength a = 0 \<longrightarrow> a = [] \<or> (\<exists>as c cs. a = Insert c cs#as)"
+  apply (induct_tac a, safe)
+  apply (case_tac a, auto)+
   done
 
-lemma operationsComplete2: "a \<in> Range operations"
-  apply (induct_tac a, force)
-  apply (case_tac a, auto)
+fun outputLength :: "'char operation \<Rightarrow> nat" where
+  "outputLength [] = 0"
+| "outputLength (Retain n#xs) = (1 + n) + outputLength xs"
+| "outputLength (Insert s ss#xs) = (1 + length ss) + outputLength xs"
+| "outputLength (Delete _#xs) = outputLength xs"
+
+text {* if an operation @{term a} has output lenght 0, @{term a} must be empty or is consists only 
+        of delete actions *}
+
+lemma emptyOutputDelete [rule_format]: "outputLength a = 0 \<longrightarrow> a = [] \<or> (\<exists>as n. a = Delete n#as)"
+  apply (induct_tac a, auto)
+  apply (case_tac a, auto)+
+  done  
+
+text {* if an operation @{term a} has output and input lenght of @{term 0}, the operation must be empty *}
+
+lemma emptyInOutOp [rule_format]: "inputLength a = 0 \<and> outputLength a = 0 \<longrightarrow> a = []"
+  apply (induct_tac a, auto)
+  apply (case_tac a, auto)+
   done
 
-fun applyOp :: "'char operation \<Rightarrow> 'char document \<Rightarrow> 'char document"
+section {* Application function *}
+
+text {* The @{term applyOp} function applies an operation @{term a} to document @{term d} and yields 
+        either @{term None} if the input length of @{term a} does not match the length of @{term d} 
+        or @{term "Some d'"} where @{term d'} is the result of a valid application *}
+
+fun splitRec :: "nat \<Rightarrow> 'char document \<Rightarrow> 'char document \<Rightarrow> ('char document \<times> 'char document) option" where
+  "splitRec 0 (y#ys) xs = Some (append xs [y],ys)"
+| "splitRec n (y#ys) xs = splitRec (n - 1) ys (append xs [y])"
+| "splitRec _ _ _ = None"
+
+definition split :: "nat \<Rightarrow> 'char document \<Rightarrow> ('char document \<times> 'char document) option" where
+  "split n ys = splitRec n ys []"
+
+fun applyOp :: "'char operation \<Rightarrow> 'char document \<Rightarrow> 'char document option"
 where
-  "applyOp ([])            ([])  = []"
-| "applyOp (Retain n#next) (doc) = append (take n doc) (applyOp next (drop n doc))"
-| "applyOp (Insert s#next) (doc) = append s (applyOp next doc)"
-| "applyOp (Delete n#next) (doc) = applyOp next (drop n doc)"
+  empty[intro!]:  "applyOp ([])               ([])  = Some []"
+| retain[intro!]: "applyOp (Retain n#next)    (doc) = Option.bind (split n doc) (\<lambda>(l,r). Option.map (append l) (applyOp next r))"
+| insert[intro!]: "applyOp (Insert c cs#next) (doc) = Option.map (append (c#cs)) (applyOp next doc)"
+| delete[intro!]: "applyOp (Delete n#next)    (doc) = Option.bind (split n doc) (\<lambda>(_,r). applyOp next r)"
+| "applyOp _                  _     = None"
 
-lemma applyOpEq: "(a,b) \<in> operations \<Longrightarrow> \<forall> d'. SimpleOperation.applyOp a d = Some d' \<longrightarrow> applyOp b d = d'" 
-  apply (rule operations.induct)
-    apply (simp)    
+subsection {* Valid Operations *}
+
+text {* iff an operation @{term a} is empty it can only be applied to the empty document and the
+        result is also the empty document *}
+
+lemma emptyInput: "applyOp [] d = Some d' \<longleftrightarrow> d = [] \<and> d' = []"  
+  by (case_tac d, auto)
+
+lemma emptyInputDomain[rule_format]: "(\<exists> d'. applyOp [] d = Some d') \<longleftrightarrow> d = []"
+  by (auto simp add: emptyInput)
+
+lemma emptyDocInsert: "\<exists>d'. applyOp (a#as) [] = Some d' \<Longrightarrow> \<exists>c cs. a = Insert c cs"
   sorry
 
-fun addRetain :: "nat \<Rightarrow> 'char operation \<Rightarrow> 'char operation" where
+text {* every document can be produced by the application of an operation to a document *}
+
+lemma applicationRange: "\<exists>a d. applyOp a d = Some d'"  
+  apply (induct_tac d')
+  apply (auto)
+  by (metis Operation.empty Operation.insert append_Nil2 option_map_Some)
+
+subsection {* In- and Output Lenghts of Valid Operations *}
+
+text {* All pairs of operations and documents are contained in the domain of the application
+        iff the inputLength of the operation matches the length of the document *}
+
+lemma applicationDomain[rule_format]: 
+  "(\<exists> d'. applyOp a d = Some d') \<longleftrightarrow> inputLength a = length d"
+  apply (induct_tac a)
+  apply (simp add: emptyInputDomain)
+  apply (case_tac a) 
+  apply (simp_all)
+  oops
+
+lemma validOutputLength: "applyOp a d = Some d' \<Longrightarrow> outputLength a = length d'"
+  oops
+
+section {* Composition of Operations *}
+
+fun addRetain :: "nat \<Rightarrow> 'char operation \<Rightarrow> 'char operation" where  
   "addRetain n (Retain m#xs) = (Retain (n + m))#xs"
 | "addRetain n xs            = (Retain n)#xs"
 
-fun addInsert :: "'char list \<Rightarrow> 'char operation \<Rightarrow> 'char operation" where
-  "addInsert s (Delete d#xs) = (Delete d)#addInsert s xs"
-| "addInsert s (Insert t#xs) = (Insert (append t s))#xs"
-| "addInsert s xs            = (Insert s)#xs"
+fun addInsert :: "'char \<Rightarrow> 'char list \<Rightarrow> 'char operation \<Rightarrow> 'char operation" where 
+  "addInsert s ss (Delete d#xs)    = (Delete d)#addInsert s ss xs"
+| "addInsert s ss (Insert c cs#xs) = (Insert c (append cs (s#ss)))#xs"
+| "addInsert s ss xs               = (Insert s ss)#xs"
 
-fun addDelete :: "nat \<Rightarrow> 'char operation \<Rightarrow> 'char operation" where
+fun addDelete :: "nat \<Rightarrow> 'char operation \<Rightarrow> 'char operation" where  
   "addDelete n (Delete m#xs) = (Delete (n + m))#xs"
 | "addDelete n xs            = (Delete n)#xs"
+
+text {* The @{term compose} function composes two operations @{term a} and @{term b}, in such a way
+        that the composed operation @{term ab} has the same effect upon application as operations
+        @{term a} and @{term b} executed sequentially. *}
 
 fun composeRec :: "'char operation \<Rightarrow> 'char operation \<Rightarrow> 'char operation \<Rightarrow> 'char operation" where
   "composeRec [] [] xs  = xs" 
 | "composeRec ((Delete n)#as) (bb) xs = composeRec as bb (addDelete n xs)"
-| "composeRec (aa) ((Insert s)#bs) xs = composeRec aa bs (addInsert s xs)"
-| "composeRec ((Retain n)#as) ((Retain m)#bs) xs =
-   (if      (n < m) then composeRec as (Retain(m - n)#bs) (addRetain n xs)
+| "composeRec (aa) ((Insert c cs)#bs) xs = composeRec aa bs (addInsert c cs xs)"
+| "composeRec ((Retain n)#as) ((Retain m)#bs) xs = 
+   (if      (n < m) then composeRec as (Retain (m - n)#bs) (addRetain n xs)
     else if (n = m) then composeRec as bs (addRetain n xs)
-    else                 composeRec (Retain(n - m)#as) bs (addRetain n xs))"
+    else                 composeRec (Retain (n - m)#as) bs (addRetain n xs))"
 | "composeRec ((Retain n)#as) ((Delete m)#bs) xs =
    (if      (n < m) then composeRec as (Delete(m - n)#bs) (addDelete n xs)
     else if (n = m) then composeRec as bs (addDelete n xs)
     else                 composeRec (Retain(n - m)#as) bs (addDelete n xs))"
-| "composeRec ((Insert s)#as) ((Retain m)#bs) xs =
-   (if      (length s < m) then composeRec as (Delete(m - length s)#bs) (addInsert s xs)
-    else if (length s = m) then composeRec as bs (addInsert s xs)
-    else                        composeRec (Insert(drop m s)#as) bs (addInsert (take m s) xs))"
-| "composeRec ((Insert s)#as) ((Delete m)#bs) xs =
-   (if      (length s < m) then composeRec as (Delete(m - length s)#bs) xs
-    else if (length s = m) then composeRec as bs xs
-    else                        composeRec (Insert(drop m s)#as) bs xs)"
+| "composeRec ((Insert c cs)#as) ((Retain m)#bs) xs =
+   (if      (length cs < m) then composeRec as (Delete(m - length cs)#bs) (addInsert c cs xs)
+    else if (length cs = m) then composeRec as bs (addInsert c cs xs)
+    else                         composeRec (Insert c (drop m cs)#as) bs (addInsert c (take m cs) xs))"
+| "composeRec ((Insert c cs)#as) ((Delete m)#bs) xs =
+   (if      (length cs < m) then composeRec as (Delete(m - length cs)#bs) xs
+    else if (length cs = m) then composeRec as bs xs
+    else                         composeRec (Insert c (drop m cs)#as) bs xs)"
+| "composeRec _ _ _ = undefined"
 
 definition compose :: "'char operation \<Rightarrow> 'char operation \<Rightarrow> 'char operation" where
   "compose a b = composeRec a b []"
 
-lemma composeEq: "(a, b) \<in> operations \<Longrightarrow> 
-                  (a', b') \<in> operations \<Longrightarrow> 
-                  SimpleOperation.compose a a' = Some a'' \<Longrightarrow> 
-                  (a'', Operation.compose b b') \<in> operations"
-  sorry
+section {* Operation Transformation *}
+
+text {* The transformation function is the basis of operational transformation. For a pair of 
+        operations @{term "(a,b)"} it computes an output pair of transformed operations 
+        @{term "(a',b')"}. The convergence property @{term "compose a b' = compose b a'"} enables
+        the OT system to execute operations in different order at different sites while the 
+        documents do not diverge *}
 
 fun transformRec :: "'char operation \<Rightarrow> 'char operation \<Rightarrow> 'char operation \<Rightarrow> 'char operation \<Rightarrow> 'char operation \<times> 'char operation" where
   "transformRec [] [] xs ys = (xs,ys)"
-| "transformRec (Insert s#as) bs xs ys = transformRec as bs (addInsert s xs) (addRetain (length s) ys)"
-| "transformRec as (Insert s#bs) xs ys = transformRec as bs (addRetain (length s) xs) (addInsert s ys)"
+| "transformRec (Insert c cs#as) bs xs ys = transformRec as bs (addInsert c cs xs) (addRetain (length cs) ys)"
+| "transformRec as (Insert c cs#bs) xs ys = transformRec as bs (addRetain (length cs) xs) (addInsert c cs ys)"
 | "transformRec (Retain n#as) (Retain m#bs) xs ys = 
    (if      (n < m) then transformRec as ((Retain (m - n))#bs) (addRetain n xs) (addRetain n ys)
     else if (n = m) then transformRec as bs (addRetain n xs) (addRetain n ys)
@@ -109,16 +210,10 @@ fun transformRec :: "'char operation \<Rightarrow> 'char operation \<Rightarrow>
    (if      (n < m) then transformRec as ((Retain (m - n))#bs) (addDelete n xs) ys
     else if (n = m) then transformRec as bs (addDelete n xs) ys
     else                 transformRec ((Delete (n - m))#as) bs (addDelete m xs) ys)"
+| "transformRec _ _ _ _ = undefined"
 
 definition transform :: "'char operation \<Rightarrow> 'char operation \<Rightarrow> ('char operation \<times> 'char operation)" where
   "transform a b = transformRec a b [] []"
-
-lemma transformEq: "(a, a') \<in> operations \<Longrightarrow>
-                    (b, b') \<in> operations \<Longrightarrow>
-                    SimpleOperation.transform a b = Some (c,d) \<Longrightarrow> 
-                    (c, fst (Operation.transform a' b')) \<in> operations \<and>
-                    (d, snd (Operation.transform a' b')) \<in> operations"
-  sorry
 
 export_code applyOp compose transform in Scala
   module_name Operation
